***NO_CI*** adding more stuff to freezing array, hooked it up with the protocol

examples/preorders/FreezingArray.fst
@@ -93,10 +93,16 @@ type index (#a:Type0) (#n:nat) (arr:array a n) = i:nat{i < n}
  * Ghost view of an array as a sequence of options
  *)
 abstract let as_seq (#a:Type0) (#n:nat) (arr:array a n) (h:heap)
-  :GTot (s:Seq.seq (option a){Seq.length s = n})
+  :GTot (s:Seq.seq (option a))
   = let A #_ #_ #_ s_ref off = arr in
     let s = fst (sel h s_ref) in
     Seq.slice s off (off + n)
+
+let lemma_as_seq_length (#a:Type0) (#n:nat) (arr:array a n) (h:heap)
+  :Lemma (requires True)
+         (ensures  (Seq.length (as_seq arr h) = n))
+	 [SMTPat (Seq.length (as_seq arr h))]
+  = ()
 
 (*
  * a sequence of option a is equivalent to a sequence of a, if all are Some and contained values match
@@ -104,6 +110,12 @@ abstract let as_seq (#a:Type0) (#n:nat) (arr:array a n) (h:heap)
 let equivalent_seqs (#a:Type0) (s1:Seq.seq (option a)) (s2:Seq.seq a) :Type0
   = (Seq.length s1 == Seq.length s2) /\
     (forall (i:nat). i < Seq.length s1 ==> Some (Seq.index s2 i) == Seq.index s1 i)
+
+let equivalent_seqs_lemma (#a:Type0) (s1:Seq.seq (option a)) (s2:Seq.seq a)
+  :Lemma (requires (equivalent_seqs s1 s2))
+         (ensures  (forall (i:nat). i < Seq.length s1 ==> Some? (Seq.index s1 i)))
+	 [SMTPat (equivalent_seqs s1 s2)]
+  = ()
 
 (* scaffolding for init_at *)
 let init_at_seq (#a:Type0) (s:Seq.seq (option a)) (i:nat{i < Seq.length s}) :Type0
@@ -136,6 +148,25 @@ abstract let init_at (#a:Type0) (#n:nat) (arr:array a n) (i:index arr) :Type0
 (* assuming this function, quite straightforward, just strip out the Some *)
 assume val get_equivalent_seq (#a:Type0) (s:Seq.seq (option a){forall (i:nat). i < Seq.length s ==> Some? (Seq.index s i)})
   :Tot (r:Seq.seq a{equivalent_seqs s r})
+
+assume val lemma_equivalent_implies_slice_equivalent
+  (#a:Type0) (s1:seq (option a)) (s2:seq a{equivalent_seqs s1 s2})
+  (i:nat) (j:nat{j >= i /\ j < Seq.length s1})
+  :Lemma (requires True)
+         (ensures  (equivalent_seqs (Seq.slice s1 i j) (Seq.slice s2 i j)))
+	 [SMTPat (equivalent_seqs (Seq.slice s1 i j) (Seq.slice s2 i j))]
+
+assume val lemma_get_equivalent_commutes_with_slice
+  (#a:Type0) (s:seq (option a){forall (i:nat). i < Seq.length s ==> Some? (Seq.index s i)}) (i:nat) (j:nat{j >= i /\ j < Seq.length s})
+  :Lemma (requires True)
+         (ensures  (Seq.slice (get_equivalent_seq s) i j == get_equivalent_seq (Seq.slice s i j)))
+	 [SMTPatOr [[SMTPat (Seq.slice (get_equivalent_seq s) i j)]; [SMTPat (get_equivalent_seq (Seq.slice s i j))]]]
+
+assume val lemma_get_equivalent_sequence_slice
+  (#a:Type0) (s:seq (option a)) (i:nat) (j:nat{j >= i /\ j <= Seq.length s})
+  (s':seq a{Seq.length s' = j - i /\ (forall (k:nat). (k >= i /\ k < j) ==> Seq.index s k == Some (Seq.index s' (k - i)))})
+  :Lemma (requires True)
+         (ensures  (get_equivalent_seq (Seq.slice s i j) == s'))
 
 (* scaffolding for frozen predicate *)
 abstract let frozen_bit (#a:Type0) (#n:nat) (arr:array a n) (h:heap) :GTot bool
@@ -210,6 +241,12 @@ abstract let sub (#a:Type0) (#n:nat) (arr:array a n) (i:index arr) (len:nat{i + 
 
 let suffix (#a:Type0) (#n:nat) (arr:array a n) (i:index arr) = sub arr i (n - i)
 let prefix (#a:Type0) (#n:nat) (arr:array a n) (i:index arr) = sub arr 0 i
+
+let lemma_sub_is_slice (#a:Type0) (#n:nat) (arr:array a n) (i:index arr) (len:nat{i + len <= n}) (h:heap)
+  :Lemma (requires True)
+         (ensures  (as_seq (sub arr i len) h == Seq.slice (as_seq arr h) i (i + len)))
+	 [SMTPat (as_seq (sub arr i len) h)]
+  = ()
 
 (*
  * footprint of a subarray is same as the footprint of the array
@@ -293,3 +330,122 @@ let lemma_frozen_implies_init_at (#a:Type0) (#n:nat) (arr:array a n) (es:erased 
          (ensures  (arr `init_at` i))
 	 [SMTPat (frozen_with arr es); SMTPat (arr `init_at` i)]
   = lemma_functoriality (frozen_pred arr es) (init_at_pred arr i)
+
+(***** some utility functions *****)
+
+let all_init_i_j (#a:Type0) (#n:nat) (arr:array a n) (i:nat) (j:nat{j >= i /\ j <= n}) :Type0
+  = forall (k:nat). k >= i /\ k < j ==> arr `init_at` k
+
+let all_init (#a:Type0) (#n:nat) (arr:array a n) :Type0
+  = all_init_i_j arr 0 n
+
+type iarray_i_j (a:Type0) (n:nat) (i:nat) (j:nat{j >= i /\ j <= n}) :Type0
+  = arr:array a n{all_init_i_j arr i j}
+
+type iarray (a:Type0) (n:nat) :Type0 = iarray_i_j a n 0 n
+
+abstract let recall_all_init_i_j (#a:Type0) (#n:nat) (arr:array a n) (i:nat) (j:nat{j >= i /\ j <= n /\ all_init_i_j arr i j})
+  :ST unit (requires (fun _ -> True))
+           (ensures  (fun h0 _ h1 -> h0 == h1 /\ (forall (k:nat). k >= i /\ k < j ==> Some? (Seq.index (as_seq arr h0) k))))
+  = let rec aux (curr:nat{curr >= i /\ curr < j})
+      :ST unit (requires (fun h0      -> forall (k:nat). k >= i /\ k < curr ==> Some? (Seq.index (as_seq arr h0) k)))
+               (ensures  (fun h0 _ h1 -> h0 == h1 /\ (forall (k:nat). k >= i /\ k < j ==> Some? (Seq.index (as_seq arr h0) k))))
+      = gst_recall (init_at_pred arr curr);
+        if curr = j - 1 then () else aux (curr + 1)
+    in
+    if i = j then ()
+    else aux i
+
+abstract let recall_all_init (#a:Type0) (#n:nat) (arr:array a n{all_init arr})
+  :ST unit (requires (fun _ -> True))
+           (ensures  (fun h0 _ h1 -> h0 == h1 /\ (forall (i:nat). i < n ==> Some? (Seq.index (as_seq arr h0) i))))
+  = recall_all_init_i_j arr 0 n
+
+abstract let witness_all_init_i_j (#a:Type0) (#n:nat) (arr:array a n) (i:nat) (j:nat{j >= i /\ j <= n})
+  :ST unit (requires (fun h0      -> forall (k:nat). k >= i /\ k < j ==> Some? (Seq.index (as_seq arr h0) k)))
+           (ensures  (fun h0 _ h1 -> h0 == h1 /\ all_init_i_j arr i j))
+  = let rec aux (curr:nat{curr >= i /\ curr < j})
+      :ST unit (requires (fun h0      -> (forall (k:nat). k >= i /\ k < j ==> Some? (Seq.index (as_seq arr h0) k)) /\ all_init_i_j arr i curr))
+               (ensures  (fun h0 _ h1 -> h0 == h1 /\ all_init_i_j arr i j))
+      = recall_contains arr;
+        gst_witness (init_at_pred arr curr);
+        if curr = j - 1 then () else aux (curr + 1)
+    in
+    if i = j then ()
+    else aux i
+
+abstract let witness_all_init (#a:Type0) (#n:nat) (arr:array a n)
+  :ST unit (requires (fun h0 -> forall (k:nat). k < n ==> Some? (Seq.index (as_seq arr h0) k)))
+           (ensures  (fun h0 _ h1 -> h0 == h1 /\ all_init arr))
+  = witness_all_init_i_j arr 0 n
+
+let as_initialized_seq (#a:Type0) (#n:nat) (arr:array a n) (h:heap{forall (i:nat). i < n ==> Some? (Seq.index (as_seq arr h) i)})
+  :GTot (seq a)
+  = let s = as_seq arr h in
+    get_equivalent_seq s
+
+let lemma_as_initialized_seq_gives_equivalent_seq
+  (#a:Type0) (#n:nat) (arr:array a n) (h:heap{forall (i:nat). i < n ==> Some? (Seq.index (as_seq arr h) i)})
+  :Lemma (requires True)
+         (ensures  (equivalent_seqs (as_seq arr h) (as_initialized_seq arr h)))
+	 [SMTPat (as_initialized_seq arr h)]
+  = ()
+
+let as_initialized_subseq (#a:Type0) (#n:nat) (arr:array a n) (h:heap)
+  (i:nat) (j:nat{j >= i /\ j <= n /\ (forall (k:nat). k >= i /\ k < j ==> Some? (Seq.index (as_seq arr h) k))})
+  :GTot (seq a)
+  = let s = as_seq arr h in
+    let s = Seq.slice s i j in
+    get_equivalent_seq s
+
+(* let lemma_as_initialized_subseq (#a:Type0) (#n:nat) (arr:array a n) (h:heap{forall (i:nat). i < n ==> Some? (Seq.index (as_seq arr h) i)}) *)
+(*   (i:nat) (j:nat{j >= i /\ j <= n}) *)
+(*   :Lemma (requires True) *)
+(*          (ensures  (let s = as_initialized_subseq arr h i j in *)
+(* 	            Seq.length s = j - i /\ s == Seq.slice (as_initialized_seq arr h) i j)) *)
+(* 	 [SMTPat (as_initialized_subseq arr h i j)] *)
+(*   = () *)
+
+abstract let read_subseq_i_j (#a:Type0) (#n:nat) (arr:array a n) (i:nat) (j:nat{j >= i /\ j <= n})
+  :ST (seq a)
+      (requires (fun h0      -> all_init_i_j arr i j))
+      (ensures  (fun h0 s h1 -> h0 == h1                                                          /\
+                             (forall (k:nat). k >= i /\ k < j ==> Some? (Seq.index (as_seq arr h0) k)) /\
+                             s == as_initialized_subseq arr h0 i j))
+  = let A #_ #_ #_ s_ref off = arr in
+    let (s, _) = !s_ref in
+    let s = Seq.slice s off (off + n) in
+    recall_all_init_i_j arr i j;
+    let s = Seq.slice s i j in
+    let s = get_equivalent_seq s in
+    s
+
+assume val copy_seq (#a:Type0) (s1:seq (option a)) (i:nat) (j:nat) (s2:seq a)
+  :Pure (seq (option a))
+        (requires (j >= i /\ j <= Seq.length s1 /\ Seq.length s2 = j - i))
+	(ensures  (fun r -> j >= i /\ j <= Seq.length s1 /\ Seq.length s2 = j - i /\
+	                 Seq.length r == Seq.length s1 /\
+                         (forall (k:nat). (k < i ==> (Seq.index r k == Seq.index s1 k)) /\
+			            ((k >= i /\ k < j) ==> (Seq.index r k == Some (Seq.index s2 (k - i)))) /\
+				    ((k >= j /\ k < Seq.length s1) ==> (Seq.index r k == Seq.index s1 k)))))
+	                 //get_equivalent_seq (Seq.slice r i j) == s2))
+
+abstract let fill (#a:Type0) (#n:nat) (arr:array a n) (buf:seq a{Seq.length buf <= n})
+  :ST unit (requires (fun h0      -> is_mutable arr h0))
+           (ensures  (fun h0 _ h1 -> modifies (array_footprint arr) h0 h1                                  /\
+	                          all_init_i_j arr 0 (Seq.length buf)                                   /\
+				  (forall (k:nat). k < Seq.length buf ==> Some? (Seq.index (as_seq arr h1) k)) /\
+				  buf == as_initialized_subseq arr h1 0 (Seq.length buf)                /\
+				  is_mutable arr h1))
+  = let A #_ #_ #m s_ref off = arr in
+    let (s, b) = !s_ref in
+    let s1 = copy_seq s off (off + Seq.length buf) buf in
+    s_ref := (s1, b);
+    witness_all_init_i_j arr 0 (Seq.length buf);
+    lemma_get_equivalent_sequence_slice s1 off (off + Seq.length buf) buf
+    
+let lemma_framing_of_is_mutable (#a:Type0) (#n:nat) (arr:array a n) (h0:heap) (h1:heap) (r:Set.set nat)
+  :Lemma (requires (modifies r h0 h1 /\ Set.disjoint r (array_footprint arr) /\ h0 `contains_array` arr /\ is_mutable arr h0))
+         (ensures  (is_mutable arr h1))
+	 [SMTPat (modifies r h0 h1); SMTPat (is_mutable arr h0)]
+  = ()
